src/DEC1/Hoare_initVAddrTable_SynDir.v
@@ -1,0 +1,836 @@
+(* Paolo Torrini, with Mohamed Sami Cherif 
+   Universite' Lille-1 - CRIStAL-CNRS
+*)
+(* verification of the initVAddrTable invariant, syntax directed version *)
+
+Require Export EnvLibA.
+Require Export RelLibA.
+Require Export PRelLibA.
+
+Require Export Coq.Program.Equality.
+Require Import Coq.Init.Specif.
+Require Import Coq.Arith.PeanoNat.
+Require Import Omega Bool Coq.Logic.ProofIrrelevance.
+Require Import Coq.Lists.List.
+
+Require Import StaticSemA.
+Require Import DynamicSemA.
+Require Import TRInductA.
+Require Import WeakenA.
+Require Import TSoundnessA.
+Require Import IdModTypeA.
+Require Import IdModPip.
+Require Import DetermA.
+Require Import AbbrevA.
+Require Import HoareA.
+Require Import THoareA.
+Require Import Lib.
+Require Import Pip_state.
+Require Import Pip_stateLib.
+Require Import Coq.Structures.Equalities.
+Require Import Coq.Logic.Eqdep.
+Require Import Hoare_getFstShadow.
+Require Import Hoare_writeVirtualInv.
+Require Import Hoare_initVAddrTable.
+Require Import Pip_DependentTypeLemmas.
+Require Import Pip_InternalLemmas.
+Require Import Pip_Prop.
+Import ListNotations.
+
+Module Hoare_Test_SndShadow_SynDir.
+
+Module SndShadowI := Hoare_Test_SndShadow.
+Export SndShadowI.
+
+(**************************************************)
+
+Definition initVAddrTableFun (fenv: funEnv)
+           (p:page) (n: nat) : Fun :=
+        FC fenv
+           [("x",Index)]
+           (Val (cst unit tt))
+           (initVAddrTableAux "initVAddrTable" "x" p)
+           "initVAddrTable"
+           n.    
+
+Lemma initVAddrTableFun_FunTyping (ftenv: funTC) (fenv: funEnv)
+      (k: MatchEnvsT FunTyping fenv ftenv)
+      (p:page) (n: nat) :
+  FunTyping (initVAddrTableFun fenv p n) (FT [("x",Index)] Unit). 
+  induction n.
+  econstructor.
+  exact k.
+  econstructor.
+  econstructor.
+  reflexivity.
+  econstructor.
+
+  econstructor.
+  exact k.
+  unfold initVAddrTableAux at 2.
+
+  econstructor.
+  unfold WriteVirtual'.
+  econstructor.
+  econstructor.
+  econstructor.
+  econstructor.
+  simpl.
+  reflexivity.
+
+  econstructor.
+  econstructor.
+  econstructor.
+  econstructor.
+  econstructor.
+  reflexivity.
+
+  econstructor.
+  econstructor.
+  econstructor.
+  econstructor.
+  econstructor.
+  econstructor.
+  econstructor.
+  reflexivity.
+
+  econstructor.
+  econstructor.
+  repeat econstructor.
+
+  econstructor.
+  reflexivity.
+  econstructor.
+  assumption.
+  assumption.
+
+  econstructor.
+  econstructor.
+  econstructor.
+  econstructor.
+
+  repeat econstructor.
+  econstructor.
+  econstructor.
+  econstructor.
+  repeat econstructor.
+
+  econstructor.
+  econstructor.
+  econstructor.
+  simpl.
+  reflexivity.
+
+  econstructor.
+  econstructor.
+  repeat econstructor.
+  econstructor.
+
+  reflexivity.
+  econstructor.
+  assumption.
+  assumption.
+  econstructor.
+  econstructor.
+  eassumption.
+  instantiate (1:=nil).
+  instantiate (1:=nil).
+  econstructor.
+  exact k.
+  simpl.
+  auto.
+  simpl.
+  reflexivity.
+  simpl.
+  reflexivity.
+
+  econstructor.
+  econstructor.
+  econstructor.
+  econstructor.
+  econstructor.
+  econstructor.
+  simpl.
+  reflexivity.
+  econstructor.
+  econstructor.
+  repeat econstructor.
+  assumption.
+Qed.  
+
+         
+Definition initVAddrTableR (p:page) (i:index) : Exp := 
+Apply
+  (QF (initVAddrTableFun nil p tableSize))
+  (PS[Val (cst index i)]).
+
+
+(******* Useful Lemmas *)
+
+Lemma succDWp2 (x:Id) P (fenv: funEnv) (env: valEnv) :
+  forall (idx:index), {{fun s => P s  /\ idx < tableSize - 1}}
+                        fenv >> (x,(cst index idx))::env >> SuccD x 
+  {{fun (idxsuc : Value) (s : state) => P s  /\ idx < tableSize - 1
+                /\ idxsuc = cst (option index) (succIndexInternal idx)
+                /\ exists i, idxsuc = cst (option index) (Some i)}}.
+Proof.
+intros.
+eapply weakenEval.
+eapply succDW.
+intros.
+simpl.
+split.
+instantiate (1:=idx).  
+intuition.
+intros.
+intuition.
+destruct idx.
+exists (CIndex (i + 1)).
+f_equal.
+unfold succIndexInternal.
+case_eq (lt_dec i tableSize).
+intros.
+auto.
+intros.
+contradiction.
+Qed.
+
+
+Lemma init_aux1 (table : page)
+  (curidx : index)
+  (fenv : funEnv)
+  (env : valEnv)
+  (H : tableSize + curidx >= tableSize) :
+  {{fun s : DynamicI.W =>
+    forall idx : index,
+    idx < curidx -> readVirtual table idx (memory s) = Some defaultVAddr
+  }}' fenv >> env >> PS [Val (cst index curidx)]
+  {{fun (vs : list Value) (s : DynamicI.W) =>
+    (forall idx : index,
+     idx < curidx -> readVirtual table idx (memory s) = Some defaultVAddr) /\
+    vs = [cst index curidx] }}'.
+
+unfold THoarePrmsTriple_Eval.
+intros.
+inversion X;subst.
+destruct vs; inversion H6.
+destruct vs ; inversion H3 ; subst.
+intuition.
+inversion X0;subst.
+inversion X2.
+inversion X2.
+Qed.
+
+Lemma init_aux01 (table : page)
+  (curidx : index)
+  (fenv : funEnv)
+  (env : valEnv)
+  (idx : index) :
+  {{fun s : DynamicI.W =>
+    idx < curidx -> readVirtual table idx (memory s) = Some defaultVAddr
+  }}' fenv >> env >> PS [Val (cst index curidx)]
+  {{fun (vs : list Value) (s : DynamicI.W) =>
+    (
+     idx < curidx -> readVirtual table idx (memory s) = Some defaultVAddr) /\
+    vs = [cst index curidx] }}'.
+
+unfold THoarePrmsTriple_Eval.
+intros.
+inversion X; subst.
+destruct vs; inversion H5.
+destruct vs ; inversion H2 ; subst.
+intuition.
+inversion X0;subst.
+inversion X2.
+inversion X2.
+Qed.
+
+
+Lemma init_aux2 (idx: index) :
+  idx < CIndex (tableSize - 1) \/ idx = CIndex (tableSize - 1).
+      destruct idx. simpl in *. 
+      unfold CIndex.
+      case_eq (lt_dec (tableSize - 1) tableSize).
+      intros. simpl in *.
+      assert (i <= tableSize -1).
+      omega.
+      apply NPeano.Nat.le_lteq in H0.
+      destruct H0.
+      left. assumption. right.
+      subst.
+      assert (Hi =  Pip_state.CIndex_obligation_1 (tableSize - 1) l).
+      apply proof_irrelevance.
+      subst. reflexivity.
+      intros.
+      intuition.
+Qed.      
+
+
+Lemma init_aux3 (* for the 'false case' *)
+ (table : page)
+ (curidx : index)
+ (fenv : funEnv)
+ (env : valEnv)
+ (e : Exp)
+ (k0 : curidx >= 0)
+ (k1 : curidx = CIndex (tableSize - 1)) :  
+  {{fun s : DynamicI.W =>
+    (forall idx : index,
+     idx < curidx -> readVirtual table idx (memory s) = Some defaultVAddr) 
+     /\ readVirtual table curidx (memory s) = Some defaultVAddr  
+  }}
+    fenv >> env >> Val (cst unit tt) 
+  {{fun (_ : Value) (s : DynamicI.W) =>
+      forall idx : index, readVirtual table idx (memory s) = Some defaultVAddr
+  }}.
+intros.
+unfold THoareTriple_Eval.
+intros.
+simpl in *.
+assert (idx < CIndex (tableSize - 1) \/ idx = CIndex (tableSize - 1)).
+eapply init_aux2.
+simpl in *.
+inversion X; subst.
+Focus 2.
+inversion X0. 
+destruct H.
+destruct H0.
+eapply H.
+exact H0.
+subst.
+exact H1.
+Qed.
+
+
+Lemma init_aux5 (table : page)
+  (idx : index)
+  (curidx : index)
+  (fenv : funEnv) :
+  {{fun s : DynamicI.W =>
+    idx < curidx -> readVirtual table idx (memory s) = Some defaultVAddr}} 
+  fenv >>
+  [("x", cst index curidx)] >> WriteVirtual' table "x" defaultVAddr
+  {{fun (_ : Value) (s : state) =>
+    (idx < curidx -> readVirtual table idx (memory s) = Some defaultVAddr) /\
+    readVirtual table curidx (memory s) = Some defaultVAddr}}.
+unfold WriteVirtual'.
+eapply Modify_VHTT3 with (fenv:= fenv)
+                         (env:=[("x", cst index curidx)])
+                         (XF:=(xf_writeVirtual' table defaultVAddr))
+                         (x:="x").
+Unshelve.
+Focus 3.
+exact curidx.
+intros.
+simpl.
+split.
+intros.
+
+unfold readVirtual.
+unfold add.
+simpl.
+assert (Hfalse :
+    Lib.beqPairs (table, curidx) (table, idx) beqPage beqIndex = false).
+    { apply beqPairsFalse. 
+      right.
+      apply indexDiffLtb.
+      right; assumption. }
+rewrite Hfalse at 1.
+assert (lookup table idx (Lib.removeDup table curidx (memory s)
+                                            beqPage beqIndex)
+               beqPage beqIndex =
+        Lib.lookup  table idx  (memory s) beqPage beqIndex) as Hmemory.
+    { apply removeDupIdentity.
+      right. 
+      apply indexDiffLtb.
+      left; trivial. }
+rewrite Hmemory.
+apply H in H0.
+unfold readVirtual in *.
+auto.
+
+unfold writeVirtualInternal.
+simpl.
+unfold readVirtual.
+unfold add.
+simpl.
+assert (Htrue : Lib.beqPairs (table, curidx) (table, curidx)
+                             beqPage beqIndex = true).
+    { apply beqPairsTrue.
+      intuition. }
+rewrite Htrue.
+auto.
+reflexivity.
+Qed.
+
+
+Lemma init_aux6 (table : page)
+  (idx : index)
+  (curidx : index)
+  (fenv : funEnv) : 
+  {{fun s : state =>
+    (idx < curidx -> readVirtual table idx (memory s) = Some defaultVAddr) /\
+    readVirtual table curidx (memory s) = Some defaultVAddr}} 
+  fenv >>
+  [("x", cst index curidx)] >> LtLtb "x" maxIndex
+  {{fun (b : Value) (s : DynamicI.W) =>
+    (idx < curidx -> readVirtual table idx (memory s) = Some defaultVAddr) /\
+    readVirtual table curidx (memory s) = Some defaultVAddr /\
+    b = cst bool (Index.ltb curidx maxIndex)}}.
+unfold LtLtb.
+eapply Modify_VHTT3 with (fenv:= fenv)
+                         (env:=[("x", cst index curidx)])
+                         (XF:=(xf_Ltb maxIndex))
+                         (x:="x").
+
+Unshelve.
+Focus 3.
+exact curidx.
+
+intros.
+destruct H.
+split.
+intuition.
+intuition.
+reflexivity.
+Qed.
+
+
+Lemma init_aux7 (table : page)
+  (idx : index)
+  (curidx : index)
+  (fenv : funEnv) :
+  {{fun s : DynamicI.W =>
+    (idx < curidx -> readVirtual table idx (memory s) = Some defaultVAddr) /\
+    readVirtual table curidx (memory s) = Some defaultVAddr /\
+    cst bool true = cst bool (Index.ltb curidx maxIndex)}}
+ fenv >> [("x", cst index curidx)] >> SuccD "x"
+  {{(fun (idxsuc : Value) (s : state) =>
+    (fun s0 : DynamicI.W =>
+     (fun s' : state =>
+      (idx < curidx -> readVirtual table idx (memory s') = Some defaultVAddr) /\
+      readVirtual table curidx (memory s0) = Some defaultVAddr) s0) s /\
+    curidx < tableSize - 1 /\
+    idxsuc = cst (option index) (succIndexInternal curidx) /\
+    (exists i : index, idxsuc = cst (option index) (Some i)))}}. 
+eapply weakenEval.
+eapply succDWp2.
+simpl;intros; intuition.
+
+unfold maxIndex in H2.
+inversion H2.
+apply inj_pair2 in H3.
+symmetry in H3.
+apply indexltbTrue in H3.
+unfold CIndex in H3.
+destruct (lt_dec (tableSize - 1) tableSize). 
+simpl in *.  
+assumption.
+contradict n.
+assert (tableSize > tableSizeLowerBound).
+apply tableSizeBigEnough.
+unfold tableSizeLowerBound in *.
+omega.
+Qed.
+
+Lemma init_aux8 (table : page)
+  (idx : index)
+  (curidx : index)
+  (fenv : funEnv)
+  (v : Value) :
+  {{fun s : state =>
+    ((idx < curidx -> readVirtual table idx (memory s) = Some defaultVAddr) /\
+     readVirtual table curidx (memory s) = Some defaultVAddr) /\
+    curidx < tableSize - 1 /\
+    v = cst (option index) (succIndexInternal curidx) /\
+    (exists i : index, v = cst (option index) (Some i))}}
+   fenv >>
+  [("idx", v);
+  ("x", cst index curidx)] >> ExtractIndex "idx"
+  {{fun (v0 : Value) (s : DynamicI.W) =>
+    (fun (v' : Value) (s0 : W) =>
+     ((idx < curidx -> readVirtual table idx (memory s0) = Some defaultVAddr) /\
+      readVirtual table curidx (memory s0) = Some defaultVAddr /\
+      curidx < tableSize - 1) /\
+     v' = cst index (match succIndexInternal curidx with | Some i => i
+                                                 | None => index_d end)) v0 s}}.
+
+eapply Hoare_env_subst with (fenv:=fun _ => fenv)
+           (env:=fun v => [("idx", v); ("x", cst index curidx)])
+           (v2:=cst (option index) (succIndexInternal curidx))
+      (P2 := (fun s : state =>
+    ((idx < curidx -> readVirtual table idx (memory s) = Some defaultVAddr) /\
+     readVirtual table curidx (memory s) = Some defaultVAddr) /\
+    curidx < tableSize - 1 /\
+    (exists i : index,
+        cst (option index) (succIndexInternal curidx) =
+        cst (option index) (Some i)))).      
+intuition.
+intuition.
+subst.
+assumption.
+
+unfold ExtractIndex.
+
+eapply Modify_VHTT3 with (fenv:= fenv)
+       (env:= [("idx", cst (option index) (succIndexInternal curidx));
+  ("x", cst index curidx)])
+                         (XF:=(xf_ExtractIndex))
+                         (x:="idx").
+
+Unshelve.
+Focus 3.
+exact (succIndexInternal curidx).
+intros.
+destruct H.
+destruct H.
+destruct H0.
+destruct H2.
+inversion H2; subst.
+repeat apply inj_pair2 in H4.
+rewrite H4 in *.
+
+unfold b_eval, b_exec, xf_ExtractIndex, b_mod in *.
+simpl in *.
+
+intuition.
+reflexivity.
+Qed.
+
+
+Lemma init_aux9 (table : page)
+  (idx : index)
+  (curidx : index)
+  (fenv : funEnv)
+  (env : valEnv) :
+  {{fun s : DynamicI.W =>
+    (idx < curidx -> readVirtual table idx (memory s) = Some defaultVAddr) /\
+    readVirtual table curidx (memory s) = Some defaultVAddr /\
+    cst bool false = cst bool (Index.ltb curidx maxIndex)}} 
+  fenv >>
+  env >> Val (cst unit tt)
+  {{fun (_ : Value) (s : DynamicI.W) =>
+    readVirtual table idx (memory s) = Some defaultVAddr}}.
+
+unfold THoareTriple_Eval.
+intros.
+intuition.
+inversion X; subst.
+Focus 2.
+inversion X0.
+
+clear X.
+simpl in *.
+inversion H2; subst.
+repeat eapply inj_pair2 in H3.
+symmetry in H3.
+apply indexltbFalse in H3.
+apply indexBoundEq in H3.
+
+assert (idx < CIndex (tableSize - 1) \/ idx = CIndex (tableSize - 1)) as H4.
+eapply init_aux2.
+destruct H4.
+
+subst.
+eapply H0.
+exact H1.
+
+subst.
+assumption.
+Qed.
+      
+
+Lemma init_aux10 (table : page)
+  (idx : index)
+  (curidx : index)
+  (fenv : funEnv) :
+  {{fun s : DynamicI.W =>
+    (idx < curidx -> readVirtual table idx (memory s) = Some defaultVAddr) /\
+    readVirtual table curidx (memory s) = Some defaultVAddr /\
+    curidx < tableSize - 1
+  }}' fenv >>
+  [("y",
+   cst index
+     match succIndexInternal curidx with
+     | Some i => i
+     | None => index_d
+     end); ("x", cst index curidx)] >> PS [VLift (Var "y")]
+  {{fun (vs : list Value) (s : DynamicI.W) =>
+    (idx < curidx -> readVirtual table idx (memory s) = Some defaultVAddr) /\
+    readVirtual table curidx (memory s) = Some defaultVAddr /\
+    curidx < tableSize - 1 /\
+    vs =
+    [cst index
+       match succIndexInternal curidx with
+       | Some i => i
+       | None => index_d
+       end] }}'.
+
+unfold VLift.
+eapply Prms_VHTT1.
+
+instantiate (1:=fun v s => (
+    idx < curidx -> readVirtual table idx (memory s) = Some defaultVAddr) /\
+   readVirtual table curidx (memory s) = Some defaultVAddr /\
+   curidx < tableSize - 1 /\
+   v =
+   cst index
+     match succIndexInternal curidx with
+     | Some i => i
+     | None => index_d
+     end).
+unfold THoareTriple_Eval.
+intros.
+assert ( EClosure
+        fenv
+        [("y",
+         cst index
+           match succIndexInternal curidx with
+           | Some i => i
+           | None => index_d
+           end); ("x", cst index curidx)] (Conf Exp s (Return LL (Var "y")))
+        (Conf Exp s (Val (cst index
+           match succIndexInternal curidx with
+           | Some i => i
+           | None => index_d
+           end))) ) as X2.
+econstructor.
+econstructor.
+econstructor.
+econstructor.
+reflexivity.
+econstructor.
+econstructor.
+econstructor.
+assert ((s' = s) /\ (v = cst index
+                  match succIndexInternal curidx with
+                  | Some i => i
+                  | None => index_d
+                  end)).
+eapply ExpConfluence.
+exact k3.
+exact k1.
+eauto.
+eauto.
+eauto.
+intuition; subst.
+assumption.
+assumption.
+
+unfold THoarePrmsTriple_Eval;intros.
+intuition.
+inversion X; subst.
+assumption.
+inversion X0.
+inversion X; subst.
+assumption.
+inversion X0.
+inversion X; subst.
+symmetry in H8.
+eapply map_eq_nil in H8.
+subst.
+auto.
+inversion X0.
+Qed.
+
+
+(******* Main Hoare Triple *)
+
+Lemma initVAddrTableNewProperty'
+      (table : page) (curidx : index)
+      (fenv: funEnv) (env: valEnv) :
+{{ fun s => forall idx : index, idx < curidx -> 
+                readVirtual table idx (memory s) = Some defaultVAddr }} 
+  fenv >> env >> initVAddrTableR table curidx 
+{{ fun _ s => forall idx,
+                readVirtual table idx (memory s) = Some defaultVAddr }}.
+Proof.
+
+eapply THoare_gen.
+intro idx.
+unfold initVAddrTableR.
+assert (tableSize + curidx >= tableSize) as H by omega.
+revert fenv env H.
+revert curidx.
+generalize tableSize at 1 3. 
+induction n. simpl. 
+(** begin case n=0 *)
+intros.
+destruct curidx.
+simpl in *.
+omega.
+(** env case n=0 *)
+intros; simpl.
+assert (curidx < tableSize) as k1.
+destruct curidx.
+intuition.
+(* eapply Apply_VHTT1.*)
+HoareTac1.
+eapply init_aux01.
+
+simpl in *.
+split.
+reflexivity.
+
+intro vs.
+unfold initVAddrTableAux.
+eapply Hoare_val_eq_wk with (fenv:= fun _ => [("initVAddrTable",
+                               FC [] [("x", Index)] 
+                                 (Val (cst unit tt))
+                                 (initVAddrTableAux "initVAddrTable" "x" table)
+                                 "initVAddrTable" n)])
+                         (env:= mkVEnv [("x", Index)]).
+clear vs.
+unfold mkVEnv.
+simpl.
+
+
+eapply BindN_VHTT1 with (P1:= fun s => (
+     idx < curidx -> readVirtual table idx (memory s) = Some defaultVAddr) /\ 
+     readVirtual table curidx s.(memory) = Some defaultVAddr).
+
+eapply init_aux5.
+
+(* eapply IfThenElse_VHTT1. *)
+HoareTac1.
+
+eapply init_aux6.
+simpl.
+eapply BindS_VHTT1 with (x:="y").
+eapply BindS_VHTT1 with (x:="idx").
+eapply init_aux7.
+
+intros; simpl.
+
+eapply init_aux8.
+
+Focus 2.
+eapply init_aux9.
+
+intros; simpl.
+eapply (Hoare_eq_wk Value) with
+    (fenv:= fun _ => [("initVAddrTable",
+             FC [] [("x", Index)] (Val (cst unit tt))
+               (initVAddrTableAux "initVAddrTable" "x" table) "initVAddrTable"
+               n)])
+    (env:= fun v => [("y", v); ("x", cst index curidx)])
+    (P:= fun s : DynamicI.W =>
+    (idx < curidx -> readVirtual table idx (memory s) = Some defaultVAddr) /\
+    readVirtual table curidx (memory s) = Some defaultVAddr /\
+    curidx < tableSize - 1)
+    (Q:=fun (_ : Value) (v0 : DynamicI.W) =>
+    readVirtual table idx (memory v0) = Some defaultVAddr)
+    (vs2:= cst index
+      match succIndexInternal curidx with
+      | Some i => i
+      | None => index_d
+      end).
+  
+eapply QFun_VHTT.
+econstructor.
+
+reflexivity.
+clear v. 
+eapply Apply_VHTT2.
+
+instantiate(1:=fun vs s => (
+    idx < curidx -> readVirtual table idx (memory s) = Some defaultVAddr) /\
+   readVirtual table curidx (memory s) = Some defaultVAddr /\
+   curidx < tableSize - 1 /\
+   vs =
+   [cst index
+     match succIndexInternal curidx with
+     | Some i => i
+     | None => index_d
+     end]).
+
+eapply init_aux10.
+
+intros.
+simpl in *.
+unfold initVAddrTableFun in IHn.
+
+destruct curidx.
+simpl in *.
+
+unfold THoareTriple_Eval in *.
+intros.
+destruct H0.
+destruct H1.
+destruct H2.
+simpl in *.
+
+case_eq (lt_dec i tableSize).
+intros; try contradiction.
+rewrite H4 in *.
+unfold CIndex in *.
+case_eq (lt_dec (i + 1) tableSize); intros.
+rewrite H5 in *.
+simpl in *.
+assert (Z : n+(i+1) = S(n+i)) by omega.
+
+specialize (IHn (CIndex(i+1)) [("initVAddrTable",
+               FC [] [("x", Index)] (Val (cst unit tt))
+                 (initVAddrTableAux "initVAddrTable" "x" table)
+                 "initVAddrTable" n)]
+               [("y",
+        cst index
+          {| i := i + 1; Hi := Pip_state.CIndex_obligation_1 (i + 1) l0 |});
+       ("x", cst index {| i := i; Hi := Hi |})]).
+
+assert (n + CIndex (i + 1) = S (n + i)) as k4.
+unfold CIndex.
+rewrite H5.
+simpl.
+auto.
+rewrite k4 in *.
+specialize (IHn H).
+
+eapply IHn.
+eauto.
+eauto.
+instantiate (1:=t).
+subst.
+simpl in *.
+unfold CIndex.
+rewrite H5.
+
+exact k3.
+subst.
+unfold CIndex.
+rewrite H5.
+
+exact X.
+
+intro.
+simpl in *.
+assert (Hor : idx = {| i := i; Hi := Hi |} \/ idx < {| i := i; Hi := Hi |}).
+    { simpl in *.
+      unfold CIndex in H6.
+      destruct (lt_dec (i + 1) tableSize).
+      subst.
+      simpl in *.
+      rewrite NPeano.Nat.add_1_r in H6.
+      apply lt_n_Sm_le in H6.
+      apply le_lt_or_eq in H6.
+      destruct H6.
+      right. assumption.
+      left. subst.
+      destruct idx. simpl in *.
+      subst. 
+      assert (Hi = Hi0).
+      apply proof_irrelevance.
+      subst. reflexivity. omega. }
+destruct Hor.
+subst.
+eassumption.
+apply H0; trivial.
+assert (i+1<tableSize) by omega.
+contradiction.
+
+intros.
+contradiction.
+Qed.
+
+
+End Hoare_Test_SndShadow_SynDir.
